assembly/DSet.v
@@ -1,0 +1,228 @@
+From Assembly Require Import Init.
+
+Unset Suggest Proof Using.
+
+
+(** Decidable subsets can be represented using Boolean predicates. This is
+essentially a simplified formalization of "prisms", i.e. a dual lenses. *)
+
+Section DSet_section.
+
+  (** Alas, the scope and notations must be repeated after the section.*)
+
+  Context {X: Type}.
+
+  Definition DSet := X -> bool.
+
+  Declare Scope DSet_scope.
+  Bind Scope DSet_scope with DSet.
+  Delimit Scope DSet_scope with DSet.
+
+
+  (** *** Membership and subsets *)
+
+  Definition member x (u: DSet) : Prop := u x.
+  Infix "∈" := member (at level 70) : type_scope.
+
+  (* TODO: Is it better to leave this implicit? *)
+  Global Instance member_decidable x u : Decidable (member x u).
+  Proof.
+    typeclasses eauto.
+  Qed.
+
+  Proposition extensionality u v (H: forall x, x ∈ u <-> x ∈ v) : u = v.
+  Proof.
+    extensionality x.
+    apply bool_extensionality, H.
+  Qed.
+
+  Definition subset u v := forall x, x ∈ u -> x ∈ v.
+  Infix "⊆" := subset (at level 70) : type_scope.
+
+  Instance subset_reflexive : Reflexive subset.
+  Proof.
+    intros u x. tauto.
+  Qed.
+
+  Corollary antisymmetry u v (Huv: u ⊆ v) (Hvu: v ⊆ u) : u = v.
+  Proof.
+    apply extensionality.
+    intros x.
+    split.
+    - apply Huv.
+    - apply Hvu.
+  Qed.
+
+  (* TODO: Make global? *)
+  Instance subset_transitive : Transitive subset.
+  Proof.
+    intros u v w Huv Hvw
+           x Hu.
+    apply Hvw.
+    apply Huv.
+    exact Hu.
+  Qed.
+
+  Instance subset_proper : Proper ( subset --> subset ==> impl) subset.
+  Proof.
+    intros u u' Hu
+           v v' Hv
+           H.
+    unfold flip in Hu.
+    transitivity u; [exact Hu |].
+    transitivity v; [| exact Hv].
+    exact H.
+  Qed.
+
+  Instance member_proper : Proper ( eq ==> subset ==> impl) member.
+  Proof.
+    intros x x' Hx
+           u u' Hu
+           H.
+    subst x'.
+    apply Hu.
+    exact H.
+  Qed.
+
+
+  (** *** Basics *)
+
+  Definition def (p: X -> Prop) {dec: forall x, Decidable (p x)} : DSet :=
+    fun x => as_bool (decide (p x)).
+
+  (** We have dropped the traditional subset notation for now. *)
+
+  Proposition def_spec x p {dec: forall x', Decidable (p x')} : x ∈ def p <-> p x.
+  Proof.
+    unfold def, member.
+    setoid_rewrite <- (asBool_decide (p x) (DP := dec x)) at 2.
+    destruct (decide (p x)) as [H|H]; tauto.
+  Qed.
+
+  Definition univ : DSet := def (fun _ => True).
+  Notation "'Ω'" := univ : DSet_scope.
+  Proposition univ_spec x : x ∈ Ω.
+  Proof. exact I. Qed.
+
+  Corollary univ_terminal u : u ⊆ Ω.
+  Proof.
+    intros x _. apply (univ_spec _).
+  Qed.
+
+  Definition empty : DSet := def (fun _ => False).
+  Notation "∅" := empty : DSet_scope.
+  Proposition empty_spec x : not ( x ∈ ∅ ).
+  Proof. exact id. Qed.
+
+  Corollary empty_initial u : ∅ ⊆ u.
+  Proof.
+    intros x H. exfalso. apply (empty_spec _ H).
+  Qed.
+
+  (** Required to define singleton sets. *)
+  Context {H_eqdec: EqDec X}.
+
+  Definition singleton x := def (eq x).
+  (** Since [{x}] collides with the standard notations. *)
+  Notation "!{ x }" := (singleton x) (at level 0, x at level 99) : DSet_scope.
+  Proposition singleton_spec x x' : x ∈ !{x'} <-> x = x'.
+  Proof.
+    unfold singleton. rewrite def_spec.
+    split; intro H; symmetry; exact H.
+  Qed.
+
+  Corollary refl {x} : x ∈ !{x}.
+  Proof.
+    apply singleton_spec. reflexivity.
+  Qed.
+
+  Proposition singleton_subset x u : !{x} ⊆ u <-> x ∈ u.
+  Proof.
+    unfold subset.
+    split.
+    - intros H.
+      apply (H x refl).
+    - intros H x'.
+      rewrite singleton_spec.
+      intros Hx. subst x'. exact H.
+  Qed.
+
+  Definition union (u v : DSet) := def (fun a => a ∈ u \/ a ∈ v).
+  Infix "∪" := union (at level 40, left associativity) : DSet_scope.
+  Proposition union_spec u v x : x ∈ u ∪ v <-> x ∈ u \/ x ∈ v.
+  Proof.
+    unfold union.
+    rewrite def_spec.
+    reflexivity.
+  Qed.
+
+  Instance union_proper : Proper (subset ==> subset ==> subset) union.
+  Proof.
+    intros u u' Hu
+           v v' Hv
+           x.
+    setoid_rewrite union_spec.
+    intros [H|H].
+    - left. apply Hu. exact H.
+    - right. apply Hv. exact H.
+  Qed.
+
+  (* TODO: Prove more union facts here? *)
+
+  Definition disjoint u v := forall x, not (x ∈ u /\ x ∈ v).
+  Infix "#" := disjoint (at level 50) : type_scope.
+
+  Instance disjoint_symmetric : Symmetric disjoint.
+  Proof.
+    intros u v H x [Hu Hv].
+    apply (H x).
+    split; assumption.
+  Qed.
+
+  Instance disjoint_proper : Proper (subset --> subset --> impl) disjoint.
+  Proof.
+    intros u u' Hu
+           v v' Hv
+           Huv x [Hxu Hxv].
+    apply (Huv x).
+    split;
+      [apply Hu
+      |apply Hv];
+      assumption.
+  Qed.
+
+  Proposition disjoint_not_member a u : !{a} # u <-> not (a ∈ u).
+  Proof.
+    unfold disjoint.
+    setoid_rewrite singleton_spec.
+    intuition.
+    congruence.
+  Qed.
+
+  Corollary disjoint_singeltons a a' : disjoint !{a} !{a'} <-> a <> a'.
+  Proof.
+    transitivity (not (a ∈ !{a'}));
+      [ rewrite disjoint_not_member
+      | rewrite singleton_spec ];
+      reflexivity.
+  Qed.
+
+End DSet_section.
+
+Arguments DSet : clear implicits.
+Declare Scope DSet_scope.
+Bind Scope DSet_scope with DSet.
+Delimit Scope DSet_scope with DSet.
+
+Module DSetNotations.
+
+  Infix "∈" := member (at level 70) : type_scope.
+  Infix "⊆" := subset (at level 70) : type_scope.
+  Infix "#" := disjoint (at level 50) : type_scope.
+
+  Notation "'Ω'" := univ : DSet_scope.
+  Notation "∅" := empty : DSet_scope.
+  Notation "!{ x }" := (singleton x) (at level 0, x at level 99) : DSet_scope.
+  Infix "∪" := union (at level 40, left associativity) : DSet_scope.
+
+End DSetNotations.
